Updates

CBConcrete/CBConcrete/Lib/Fin.lean
@@ -2,17 +2,36 @@ import Mathlib.Data.Fin.SuccPred
 
 namespace Fin
 
-variable {m : ℕ}
+variable {n : ℕ}
 
-theorem coe_succAbove {i : Fin m} {j : Fin (m + 1)} :
-    (j.succAbove i : ℕ) = i.val + if j.val ≤ i.val then 1 else 0 := by
+@[simp, grind =]
+theorem coe_xor {i j : Fin n} : (i ^^^ j).val = (i.val ^^^ j.val) % n := rfl
+
+@[grind =]
+theorem coe_succAbove {i : Fin n} {p : Fin (n + 1)} :
+    (p.succAbove i : ℕ) = if p.val ≤ i.val then i.val + 1 else i.val := by
   grind [succAbove, coe_castSucc, val_succ]
 
-theorem coe_predAbove {i : Fin m} {j : Fin (m + 1)} :
-    (i.predAbove j : ℕ) = j.val - (if i.val < j.val then 1 else 0) := by
+@[grind =]
+theorem coe_predAbove {p : Fin n} {i : Fin (n + 1)} :
+    (p.predAbove i : ℕ) = if p.val < i.val then i.val - 1 else i.val := by
   grind [predAbove, coe_castSucc, coe_pred, coe_castPred]
 
-@[simp]
-theorem coe_xor {i j : Fin m} : (i ^^^ j).val = (i.val ^^^ j.val) % m := rfl
+def newPredAbove (p i : Fin (n + 1)) (hip : i ≠ p) : Fin n :=
+  if h : p < i then i.pred <| p.ne_zero_of_lt h
+  else i.castPred <| i.ne_last_of_lt ((i.lt_or_lt_of_ne hip).resolve_right h)
+
+@[simp, grind =]
+theorem coe_newPredAbove {p i : Fin (n + 1)} {hip : i ≠ p} :
+    (p.newPredAbove i hip  : ℕ) = if p.val < i.val then i.val - 1 else i.val := by
+  grind [newPredAbove, coe_pred, coe_castPred]
+
+theorem predAbove_eq_newPredAbove_succAbove (p : Fin n) (i : Fin (n + 1)) :
+    p.predAbove i = newPredAbove (i.succAbove p) i (ne_succAbove _ _) := Fin.ext <| by grind
+
+theorem newPredAbove_eq_dite_castPred_predAbove {p i : Fin (n + 1)} {hip : i ≠ p} :
+    p.newPredAbove i hip = if h : p = last n then
+    i.castPred (h ▸ hip) else (p.castPred h).predAbove i := Fin.ext <| by
+  grind [val_last, coe_castPred]
 
 end Fin
