CBConcrete/CBConcrete/RemoveInsert.lean
@@ -11,90 +11,113 @@ variable {p q i j k m n : ℕ} {b b' : Bool}
 
 /-- `removeBit q i` returns the number that remains if the
   `(i+1)` least significant bit is erased from `q`.-/
-def removeBit (q i : ℕ) := ((q >>> (i + 1)) <<< i) ||| (q &&& ((1 <<< i) - 1))
+def removeBit (q i : ℕ) := ((q >>> (i + 1)) <<< i) ||| (q &&& (2^i - 1))
 
 /-- `insertBit b p i` returns the number that arises if the bit `b` is
 inserted into `p` such that it is the `(i+1)` least significant bit in the result.-/
 
 def insertBit (b : Bool) (p : ℕ) (i : ℕ) :=
-  ((p >>> i) <<< (i + 1)) ||| (p &&& ((1 <<< i) - 1)) ||| (b.toNat <<< i)
+  ((p >>> i) <<< (i + 1)) ||| (b.toNat <<< i) ||| (p &&& (2^i - 1))
 
-theorem removeBit_def : q.removeBit i = (q >>> (i + 1)) <<< i ||| q &&& ((1 <<< i) - 1) := rfl
+theorem removeBit_def : q.removeBit i = (q >>> (i + 1)) <<< i ||| q &&& (2^i - 1) := rfl
 
 theorem insertBit_def : p.insertBit b i =
-    ((p >>> i) <<< (i + 1)) ||| (p &&& ((1 <<< i) - 1)) ||| (b.toNat <<< i) := rfl
+    ((p >>> i) <<< (i + 1)) ||| (b.toNat <<< i) ||| (p &&& (2^i - 1)) := rfl
 
 -- inductive definition
-theorem removeBit_zero : q.removeBit 0 = q.div2 := by
-  simp_rw [removeBit_def, zero_add, shiftLeft_zero, tsub_self, and_zero,
-    or_zero, shiftRight_one, div2_val]
+@[grind =]
+theorem removeBit_zero : q.removeBit 0 = q / 2 := eq_of_testBit_eq <| by grind [removeBit]
+@[grind =]
+theorem insertBit_zero : q.insertBit b 0 = q.bit b := eq_of_testBit_eq <| by grind [insertBit]
 
-theorem insertBit_zero : q.insertBit b 0 = q.bit b := by
-  simp_rw [insertBit_def, shiftRight_zero, zero_add, shiftLeft_zero, tsub_self,
-    and_zero, or_zero, shiftLeft_one]
-  cases b
-  · simp_rw [Bool.toNat_false, or_zero, bit_false]
-  · simp_rw [Bool.toNat_true, or_one, div2_bit0]
+@[grind =]
+theorem removeBit_succ {q i : ℕ} : q.removeBit (i + 1) = ((q / 2).removeBit i).bit (q.testBit 0) :=
+    eq_of_testBit_eq <| by grind [removeBit]
 
-theorem removeBit_succ {q i : ℕ} : q.removeBit (i + 1) = (q.div2.removeBit i).bit q.bodd := by
-  simp_rw [removeBit_def, one_shiftLeft, and_two_pow_sub_one_eq_mod, Nat.testBit_ext_iff,
-    testBit_bit, testBit_or, testBit_shiftLeft, testBit_shiftRight, testBit_mod_two_pow]
-  rintro (_ | _)
-  · simp_rw [le_zero_iff, succ_ne_zero, if_true, zero_lt_succ, decide_true, decide_false,
-      Bool.false_and, Bool.false_or, Bool.true_and, testBit_zero_eq_bodd]
-  · simp_rw [succ_ne_zero, if_false, add_le_add_iff_right, add_lt_add_iff_right,
-      add_tsub_cancel_right, add_tsub_add_eq_tsub_right,
-      Nat.add_right_comm _ 1, testBit_succ_eq_testBit_div2]
-
+@[grind =]
 theorem insertBit_succ {q i : ℕ} :
-    q.insertBit b (i + 1) = (q.div2.insertBit b i).bit q.bodd := by
-  simp_rw [insertBit_def, one_shiftLeft,and_two_pow_sub_one_eq_mod, Nat.testBit_ext_iff, testBit_bit,
-    testBit_or, testBit_shiftLeft, testBit_shiftRight, testBit_mod_two_pow]
-  rintro (_ | _)
-  · simp_rw [le_zero_iff, succ_ne_zero, if_true, zero_lt_succ, decide_true, decide_false,
-      Bool.false_and, Bool.false_or, Bool.or_false, Bool.true_and, testBit_zero_eq_bodd]
-  · simp_rw [succ_ne_zero, if_false, add_le_add_iff_right, add_lt_add_iff_right,
-      add_tsub_cancel_right, add_tsub_add_eq_tsub_right,
-      Nat.add_right_comm _ 1, testBit_succ_eq_testBit_div2]
+    q.insertBit b (i + 1) = ((q / 2).insertBit b i).bit (q.testBit 0) := eq_of_testBit_eq <| by
+  rintro (_ | j) <;> grind [insertBit]
 
 -- basic combination eq theorems
 
 @[simp, grind =]
 theorem testBit_insertBit_of_eq {p i : ℕ} : (p.insertBit b i).testBit i = b := by
-  induction i generalizing p b with | zero | succ _ IH
-  · simp_rw [insertBit_zero, testBit_bit_zero]
-  · simp_rw [insertBit_succ, testBit_succ_eq_testBit_div2, div2_bit, IH]
+  induction i generalizing p b <;> grind
 
 @[simp, grind =]
 theorem removeBit_insertBit_of_eq {p i : ℕ} : (p.insertBit b i).removeBit i = p := by
-  induction i generalizing p b with | zero | succ _ IH
-  · simp_rw [insertBit_zero, removeBit_zero, div2_bit]
-  · simp_rw [insertBit_succ, removeBit_succ, div2_bit, bodd_bit, IH, bit_bodd_div2]
+  induction i generalizing p b <;> grind
 
 @[simp, grind =]
 theorem insertBit_testBit_removeBit_of_eq {q i : ℕ} :
     (q.removeBit i).insertBit (q.testBit i) i = q := by
-  induction i generalizing q with | zero | succ _ IH
-  · simp_rw [insertBit_zero, removeBit_zero, testBit_zero_eq_bodd, bit_bodd_div2]
-  · simp_rw [insertBit_succ, removeBit_succ, testBit_succ_eq_testBit_div2,
-      div2_bit, bodd_bit, IH, bit_bodd_div2]
+  induction i generalizing q <;> grind
+
+-- testBit_removeBit
+
+@[grind =]
+theorem testBit_removeBit {i j q : ℕ} :
+    (q.removeBit j).testBit i = q.testBit (i + (decide (j ≤ i)).toNat) := by
+  induction j generalizing q i <;> grind [cases Nat]
+
+theorem testBit_removeBit_of_lt {i j q : ℕ} (hij : i < j) :
+    (q.removeBit j).testBit i = q.testBit i := by grind
+
+theorem testBit_removeBit_of_ge {i j q : ℕ} (hij : j ≤ i) :
+    (q.removeBit j).testBit i = q.testBit (i + 1) := by grind
+
+theorem testBit_pred_removeBit_of_gt {i j q : ℕ} (hij : j < i) :
+    (q.removeBit j).testBit (i - 1) = q.testBit i := by grind
+
+theorem testBit_removeBit_succ_of_le {i j q : ℕ} (hij : i ≤ j) :
+    (q.removeBit (j + 1)).testBit i = q.testBit i := by grind
+
+-- testBit_insertBit
+
+theorem testBit_insertBit_of_lt {i j p : ℕ} (hij : i < j) :
+    (p.insertBit b j).testBit i = p.testBit i := by
+  induction j generalizing i b p <;> grind
+
+theorem testBit_insertBit_of_gt {i j p : ℕ} (hij : j < i) :
+    (p.insertBit b j).testBit i = p.testBit (i - 1) := by
+  induction j generalizing i b p <;> grind
+
+@[grind =]
+theorem testBit_insertBit {i j p : ℕ} : (p.insertBit b j).testBit i =
+    if (i = j) then b else p.testBit (i - (decide (j < i)).toNat) := by
+  split <;> grind [testBit_insertBit_of_lt, testBit_insertBit_of_gt]
+
+theorem testBit_insertBit_of_ne {i j p : ℕ} (hij : i ≠ j) : (p.insertBit b j).testBit i =
+    p.testBit (i - (decide (j < i)).toNat) := by
+  rcases hij.lt_or_gt with hij | hij
+  · simp_rw [testBit_insertBit_of_lt hij, Bool.toNat_neg (hij.not_gt), tsub_zero] ;
+  · simp only [testBit_insertBit_of_gt hij, Bool.toNat_pos hij]
+
+theorem testBit_insertBit_succ_of_le {i j p : ℕ} (hij : i ≤ j) :
+    (p.insertBit b (j + 1)).testBit i = p.testBit i := by
+  rw [testBit_insertBit_of_lt (Nat.lt_succ_of_le hij)]
+
+theorem testBit_succ_insertBit_of_ge {i j p : ℕ} (hij : j ≤ i) :
+    (p.insertBit b j).testBit (i + 1) = p.testBit i := by
+  rw [testBit_insertBit_of_gt (Nat.lt_succ_of_le hij), succ_eq_add_one, add_tsub_cancel_right]
 
 -- Equivalence family
 
-section MergeBitEquiv
+section InsertBitEquiv
 
 open Equiv
 
-@[pp_nodot, simps! symm_apply_fst symm_apply_snd apply]
+@[pp_nodot, simps! symm_apply  apply]
 def insertBitEquiv (i : ℕ) : Bool × ℕ ≃ ℕ where
   toFun bp := bp.2.insertBit bp.1 i
   invFun n := (n.testBit i, n.removeBit i)
-  left_inv _ := Prod.ext testBit_insertBit_of_eq removeBit_insertBit_of_eq
-  right_inv _ := insertBit_testBit_removeBit_of_eq
+  left_inv _ := by grind
+  right_inv _ := by grind
 
-theorem insertBitEquiv_zero : insertBitEquiv 0 = boolProdNatEquivNat := by
-  simp_rw [Equiv.ext_iff, Equiv.boolProdNatEquivNat_apply, Function.uncurry_def,
-    insertBitEquiv_apply, insertBit_zero, implies_true]
+theorem insertBitEquiv_zero : insertBitEquiv 0 = boolProdNatEquivNat := Equiv.ext <| fun _ => by
+  simp_rw [Equiv.boolProdNatEquivNat_apply, Function.uncurry_def,
+    insertBitEquiv_apply, insertBit_zero]
 
 theorem insertBitEquiv_succ : insertBitEquiv (i + 1) =
   (prodCongrRight (fun _ => (insertBitEquiv 0).symm)).trans (
@@ -104,24 +127,23 @@ theorem insertBitEquiv_succ : insertBitEquiv (i + 1) =
         (insertBitEquiv 0))))) := by
   simp_rw [Equiv.ext_iff, trans_apply, prodAssoc_symm_apply, prodCongrLeft_apply, prodComm_apply,
     Prod.swap_prod_mk, prodAssoc_apply, insertBitEquiv_apply, Prod.forall,
-    prodCongrRight_apply, insertBitEquiv_symm_apply_fst, insertBitEquiv_symm_apply_snd,
-    insertBitEquiv_apply, insertBit_succ, insertBit_zero, testBit_zero_eq_bodd,
-    removeBit_zero, implies_true]
+    prodCongrRight_apply, insertBitEquiv_symm_apply, insertBitEquiv_apply,
+    insertBit_succ, insertBit_zero, removeBit_zero, implies_true]
 
-end MergeBitEquiv
+end InsertBitEquiv
 
 -- basic application theorems
 
 theorem removeBit_apply : q.removeBit i = 2^i * (q / 2^(i + 1)) + q % 2^i := by
   induction i generalizing q with | zero | succ _ IH
-  · simp_rw [removeBit_zero, div2_val, pow_zero, zero_add, pow_one, one_mul, mod_one, add_zero]
-  · simp_rw [removeBit_succ, IH, bit_val, div2_val, bodd_toNat, pow_succ', mod_mul, mul_add,
-    mul_assoc, Nat.div_div_eq_div_mul, add_assoc, add_comm]
+  · grind
+  · simp_rw [removeBit_succ, IH]
+    grind [Nat.div_div_eq_div_mul, mod_mul]
 
 theorem insertBit_apply : p.insertBit b i = p + 2^i * ((p / 2^i) + b.toNat) := by
   induction i generalizing p b with | zero | succ _ IH
-  · simp_rw [insertBit_zero, bit_val, pow_zero, Nat.div_one, one_mul, two_mul, add_assoc]
-  · simp_rw [insertBit_succ, IH, bit_val, div2_val, bodd_toNat, pow_succ', mul_add, mul_assoc,
+  · grind
+  · simp_rw [insertBit_succ, IH, bit_val, toNat_testBit_zero, pow_succ', mul_add, mul_assoc,
       Nat.div_div_eq_div_mul, add_right_comm, Nat.div_add_mod]
 
 -- apply lemmas
@@ -150,42 +172,14 @@ theorem insertBit_apply_not {p : ℕ} : p.insertBit (!b) i =
   · rw [Bool.not_false, cond_false, insertBit_apply_false_add_pow_two]
   · rw [Bool.not_true, cond_true, insertBit_apply_true_sub_pow_two]
 
--- testBit_removeBit
-
-theorem testBit_removeBit_of_lt {i j q : ℕ} (hij : i < j) :
-    (q.removeBit j).testBit i = q.testBit i := by
-  simp_rw [removeBit_def, testBit_or, testBit_and, testBit_shiftLeft, one_shiftLeft,
-  testBit_two_pow_sub_one, hij.not_ge]
-  grind
-
-theorem testBit_removeBit_of_ge {i j q : ℕ} (hij : j ≤ i) :
-    (q.removeBit j).testBit i = q.testBit (i + 1) := by
-  simp_rw [removeBit_def, testBit_or, testBit_shiftLeft, testBit_shiftRight, add_right_comm,
-  add_tsub_cancel_of_le hij, testBit_and, one_shiftLeft, testBit_two_pow_sub_one, hij.not_gt, hij,
-  decide_true, Bool.true_and, decide_false, Bool.and_false, Bool.or_false]
-
-theorem testBit_removeBit {i j q : ℕ} :
-    (q.removeBit j).testBit i = q.testBit (i + (decide (j ≤ i)).toNat) := by
-  rcases le_or_gt j i with hij | hij
-  · rw [testBit_removeBit_of_ge hij, Bool.toNat_pos hij]
-  · rw [testBit_removeBit_of_lt hij, Bool.toNat_neg hij.not_ge, add_zero]
-
-theorem testBit_pred_removeBit_of_gt {i j q : ℕ} (hij : j < i) :
-    (q.removeBit j).testBit (i - 1) = q.testBit i := by
-  rw [testBit_removeBit_of_ge (Nat.le_sub_one_of_lt hij), Nat.sub_add_cancel (one_le_of_lt hij)]
-
-theorem testBit_removeBit_succ_of_le {i j q : ℕ} (hij : i ≤ j) :
-    (q.removeBit (j + 1)).testBit i = q.testBit i := by
-  rw [testBit_removeBit_of_lt (Nat.lt_succ_of_le hij)]
-
 -- removeBit equalities and inequalities
 
 theorem removeBit_div_two_pow_eq (h : i ≤ k) : q.removeBit i / 2^k = q / 2^(k + 1) := by
-  simp_rw [Nat.testBit_ext_iff, testBit_div_two_pow,
+  simp_rw [testBit_eq_iff, testBit_div_two_pow,
   testBit_removeBit_of_ge (h.trans (Nat.le_add_left _ _)), Nat.add_assoc, implies_true]
 
 theorem removeBit_mod_two_pow_eq (h : k ≤ i) : q.removeBit i % 2^k = q % 2^k := by
-  simp_rw [Nat.testBit_ext_iff, testBit_mod_two_pow]
+  simp_rw [testBit_eq_iff, testBit_mod_two_pow]
   intro j
   rcases lt_or_ge j k with hjk | hjk
   · simp_rw [hjk, testBit_removeBit_of_lt (hjk.trans_le h)]
@@ -212,46 +206,6 @@ theorem removeBit_lt_two_pow_iff_lt_two_pow (h : i ≤ m) : q.removeBit i < 2^m 
   have H := removeBit_lt_two_pow_mul_iff_lt_two_pow_mul h 1 (q := q)
   simp_rw [mul_one] at H
   exact H
-
--- testBit_insertBit
-
-theorem testBit_insertBit_of_lt {i j p : ℕ} (hij : i < j) :
-    (p.insertBit b j).testBit i = p.testBit i := by
-  simp only [insertBit_def, one_shiftLeft, and_two_pow_sub_one_eq_mod, testBit_or,
-    testBit_shiftLeft, ge_iff_le, (lt_succ_of_lt hij).not_ge, decide_false, testBit_shiftRight,
-    Bool.false_and, testBit_mod_two_pow, hij, decide_true, Bool.true_and, Bool.false_or,
-    hij.not_ge, Bool.or_false]
-
-theorem testBit_insertBit_of_gt {i j p : ℕ} (hij : j < i) :
-    (p.insertBit b j).testBit i = p.testBit (i - 1) := by
-  rcases Nat.exists_eq_add_of_lt hij with ⟨k, rfl⟩
-  simp_rw [insertBit_def, one_shiftLeft,
-    and_two_pow_sub_one_eq_mod, testBit_or, testBit_shiftLeft, testBit_shiftRight,
-    testBit_mod_two_pow, ← Nat.add_sub_assoc (succ_le_of_lt hij), succ_eq_add_one,
-    Nat.add_sub_add_left, succ_le_of_lt hij, add_comm j, Nat.add_right_comm _ j,
-    Nat.add_sub_cancel, testBit_toNat_succ, (Nat.le_add_left j _).not_gt, decide_true,
-    Bool.true_and, decide_false, Bool.false_and, Bool.and_false, Bool.or_false]
-
-theorem testBit_insertBit_of_ne {i j p : ℕ} (hij : i ≠ j) : (p.insertBit b j).testBit i =
-    p.testBit (i - (decide (j < i)).toNat) := by
-  rcases hij.lt_or_gt with hij | hij
-  · simp_rw [testBit_insertBit_of_lt hij, Bool.toNat_neg (hij.not_gt), tsub_zero] ;
-  · simp only [testBit_insertBit_of_gt hij, Bool.toNat_pos hij]
-
-@[grind =]
-theorem testBit_insertBit {i j p : ℕ} : (p.insertBit b j).testBit i =
-    bif (i = j) then b else p.testBit (i - (decide (j < i)).toNat) := by
-  rcases eq_or_ne i j with rfl | hij
-  · simp_rw [testBit_insertBit_of_eq, decide_true, cond_true]
-  · simp_rw [hij, testBit_insertBit_of_ne hij, decide_false, cond_false]
-
-theorem testBit_insertBit_succ_of_le {i j p : ℕ} (hij : i ≤ j) :
-    (p.insertBit b (j + 1)).testBit i = p.testBit i := by
-  rw [testBit_insertBit_of_lt (Nat.lt_succ_of_le hij)]
-
-theorem testBit_succ_insertBit_of_ge {i j p : ℕ} (hij : j ≤ i) :
-    (p.insertBit b j).testBit (i + 1) = p.testBit i := by
-  rw [testBit_insertBit_of_gt (Nat.lt_succ_of_le hij), succ_eq_add_one, add_tsub_cancel_right]
 
 -- Remaining of_eq theorems
 
@@ -346,49 +300,33 @@ theorem removeBit_le_removeBit_iff_lt_of_testBit_eq {p q : ℕ} (h : p.testBit i
 
 theorem removeBit_insertBit_of_gt {p : ℕ} (hij : j < i) :
     (p.insertBit b j).removeBit i = (p.removeBit (i - 1)).insertBit b j := by
-  simp only [Nat.testBit_ext_iff, testBit_removeBit, testBit_insertBit, tsub_le_iff_right]
+  simp only [testBit_eq_iff, testBit_removeBit, testBit_insertBit, tsub_le_iff_right]
   intro k
   rcases lt_trichotomy j (k + (decide (i ≤ k)).toNat) with hjk | rfl | hjk
   · have H : j < k := (le_or_gt i k).by_cases (lt_of_le_of_lt' · hij)
       (fun h => hjk.trans_eq (by simp_rw [h.not_ge, decide_false, Bool.toNat_false, add_zero]))
-    simp only [hjk.ne', decide_false, hjk, decide_true, Bool.toNat_true,
-      Nat.sub_add_comm (one_le_of_lt H), cond_false, H.ne', H,
-      Nat.sub_one_add_one_eq_of_pos (zero_lt_of_lt H)]
-  · simp only [decide_true, lt_self_iff_false, decide_false, Bool.toNat_false,
-      tsub_zero, cond_true, left_eq_add, Bool.toNat_eq_zero, decide_eq_false_iff_not,
-      not_le, (le_self_add).trans_lt hij, add_lt_iff_neg_left, not_lt_zero']
+    grind
+  · grind
   · have hkj : k < j := le_self_add.trans_lt hjk
-    have hik : ¬ i ≤ k + 1 := ((succ_le_of_lt hkj).trans_lt hij).not_ge
     have hik' : ¬ i ≤ k := lt_asymm hkj ∘ hij.trans_le
-    simp only [hik, hkj.not_gt, hkj.ne, hik', add_zero,
-      decide_false, Bool.toNat_false, tsub_zero, cond_false]
+    simp only [hkj.not_gt, hik']
+    grind
 
 theorem removeBit_insertBit_of_lt {p : ℕ} (hij : i < j) :
     (p.insertBit b j).removeBit i = (p.removeBit i).insertBit b (j - 1) := by
   rcases Nat.exists_eq_add_of_lt hij with ⟨j, rfl⟩
-  simp only [Nat.testBit_ext_iff, testBit_removeBit, testBit_insertBit, add_tsub_cancel_right]
+  simp only [testBit_eq_iff, testBit_removeBit, testBit_insertBit, add_tsub_cancel_right]
   intro k
   rcases le_or_gt i k with hik | hik
-  · simp only [hik, decide_true, Bool.toNat_true, add_left_inj, add_lt_add_iff_right]
-    rcases lt_trichotomy (i + j) k with hjk | rfl | hjk
-    · simp only [hjk.ne', decide_false, hjk, decide_true, Bool.toNat_true, add_tsub_cancel_right,
-      cond_false, (le_add_right _ _).trans (Nat.le_sub_one_of_lt hjk), decide_true,
-      Bool.toNat_true, Nat.sub_add_cancel (one_le_of_lt hjk)]
-    · simp only [decide_true, lt_self_iff_false, decide_false, Bool.toNat_false, tsub_zero,
-      testBit_succ, cond_true, le_add_iff_nonneg_right, _root_.zero_le, Bool.toNat_true]
-    · simp only [hjk.ne, decide_false, hjk.not_gt, Bool.toNat_false, tsub_zero, testBit_succ,
-      cond_false, hik, decide_true, Bool.toNat_true]
-  · simp only [hik.not_ge, decide_false, Bool.toNat_false, add_zero, (hik.trans hij).ne,
-      (hik.trans hij).not_gt, tsub_zero, cond_false, hik.trans_le (Nat.le_add_right _ _), ne_of_lt,
-      not_lt_of_gt]
+  · simp only [hik, decide_true, Bool.toNat_true]
+    rcases lt_trichotomy (i + j) k <;> grind
+  · grind
 
 theorem removeBit_insertBit_of_ne {p : ℕ} (hij : i ≠ j) : (p.insertBit b j).removeBit i =
     (p.removeBit (i - (decide (j < i)).toNat)).insertBit b (j - (decide (i < j)).toNat) := by
-  rcases hij.lt_or_gt with hij | hij
-  · simp only [removeBit_insertBit_of_lt hij, hij.not_gt, decide_false, Bool.toNat_false, tsub_zero,
-    hij, decide_true, Bool.toNat_true]
-  · simp only [removeBit_insertBit_of_gt hij, hij, decide_true, Bool.toNat_true, hij.not_gt,
-    decide_false, Bool.toNat_false, tsub_zero]
+  rcases hij.lt_or_gt
+  · grind [removeBit_insertBit_of_lt]
+  · grind [removeBit_insertBit_of_gt]
 
 @[grind =]
 theorem removeBit_insertBit {i j p : ℕ} : (p.insertBit b j).removeBit i = bif i = j then p else
@@ -455,7 +393,7 @@ theorem insertBit_pred_removeBit_of_gt {q : ℕ} (hij : j < i) :
 
 theorem removeBit_removeBit_of_lt {i j q : ℕ} (hij : i < j) : (q.removeBit j).removeBit i =
   (q.removeBit i).removeBit (j - 1) := by
-  simp_rw [Nat.testBit_ext_iff, testBit_removeBit, tsub_le_iff_right]
+  simp_rw [testBit_eq_iff, testBit_removeBit, tsub_le_iff_right]
   intro k
   rcases lt_or_ge k i with (hik | hik)
   · have hkj : k + 1 < j := (Nat.succ_le_of_lt hik).trans_lt hij
@@ -466,7 +404,7 @@ theorem removeBit_removeBit_of_lt {i j q : ℕ} (hij : i < j) : (q.removeBit j).
 
 theorem removeBit_removeBit_of_ge {i j q : ℕ} (hij : j ≤ i) :
     (q.removeBit j).removeBit i = (q.removeBit (i + 1)).removeBit j := by
-  simp_rw [Nat.testBit_ext_iff, testBit_removeBit]
+  simp_rw [testBit_eq_iff, testBit_removeBit]
   intro k
   rcases le_or_gt i k with (hik | hik)
   · have hjk : j ≤ k := hij.trans hik
@@ -537,11 +475,11 @@ theorem insertBit_insertBit_pred_of_lt {i j p : ℕ} {b b' : Bool} (h : i < j) :
 -- insertBit equalities and inequalities
 
 theorem insertBit_div_two_pow_eq (h : i ≤ k) : q.insertBit b i / 2^(k + 1) = q / 2^k := by
-  simp_rw [Nat.testBit_ext_iff, testBit_div_two_pow, ← Nat.add_assoc,
+  simp_rw [testBit_eq_iff, testBit_div_two_pow, ← Nat.add_assoc,
   testBit_succ_insertBit_of_ge ((h.trans (Nat.le_add_left _ _))), implies_true]
 
 theorem insertBit_mod_two_pow_eq (h : k ≤ i) : q.insertBit b i % 2^k = q % 2^k := by
-  simp_rw [Nat.testBit_ext_iff, testBit_mod_two_pow]
+  simp_rw [testBit_eq_iff, testBit_mod_two_pow]
   intro j
   rcases lt_or_ge j k with hjk | hjk
   · simp_rw [hjk, testBit_insertBit_of_lt (hjk.trans_le h)]
@@ -571,10 +509,10 @@ theorem insertBit_removeBit_lt_iff_lt (hin : 2^(i + 1) ∣ n) :
   rw [insertBit_lt_iff_lt_div_two hin, removeBit_lt_div_two_iff_lt hin]
 
 theorem zero_removeBit : (0 : ℕ).removeBit i = 0 := by
-  rw [removeBit_def, zero_shiftRight, zero_shiftLeft, zero_and, or_zero]
+  induction i <;> grind
 
 theorem zero_insertBit : (0 : ℕ).insertBit b i = b.toNat * 2^i := by
-  simp_rw [insertBit_def, zero_shiftRight, zero_shiftLeft, zero_and, or_zero, zero_or, shiftLeft_eq]
+  induction i <;> grind
 
 theorem zero_insertBit_true : (0 : ℕ).insertBit true i = 2^i := by
   simp_rw [zero_insertBit, Bool.toNat_true, one_mul]
@@ -594,13 +532,8 @@ theorem two_pow_removeBit_of_gt (hij : j < i) : (2 ^ i).removeBit j = 2 ^ (i - 1
 theorem removeBit_eq_mod_of_lt (hq : q < 2^(i + 1)) : q.removeBit i = q % 2^i := by
   cases q using Nat.bitCasesOn with | bit b q => _
   simp_rw [Nat.bit_lt_two_pow_succ_iff] at hq
-  simp_rw [Nat.testBit_ext_iff, testBit_removeBit, testBit_mod_two_pow]
-  intro j
-  rcases lt_or_ge j i with (h | h)
-  · simp_rw [h, h.not_ge, decide_true, decide_false, Bool.toNat_false, add_zero, Bool.true_and]
-  · simp_rw [h, h.not_gt, decide_true, decide_false, Bool.toNat_true, Bool.false_and,
-      testBit_succ_eq_testBit_div2, div2_bit]
-    exact Nat.testBit_lt_two_pow (hq.trans_le (Nat.pow_le_pow_of_le one_lt_two h))
+  simp_rw [testBit_eq_iff]
+  grind
 
 theorem removeBit_eq_of_lt (hq : q < 2^i) : q.removeBit i = q := by
   rw [removeBit_eq_mod_of_lt (hq.trans (Nat.pow_lt_pow_of_lt one_lt_two (Nat.lt_succ_self _))),
@@ -612,3 +545,90 @@ theorem two_pow_insertBit_false (hq : q < 2^j) : q.insertBit false j = q := by
 end RemoveInsert
 
 end Nat
+
+namespace Fin
+
+end Fin
+
+namespace BitVec
+open Nat
+
+variable {w} {b : Bool} {q : BitVec (w + 1)} {p : BitVec w} {i : Fin (w + 1)}
+
+@[simps!]
+def insertLsb (b : Bool) (p : BitVec w) (i : Fin (w + 1)) : BitVec (w + 1) :=
+  BitVec.ofNatLT (p.toNat.insertBit b i) <|
+  (Nat.insertBit_lt_two_pow_iff_lt_two_pow i.is_le).mpr p.isLt
+
+@[grind =]
+theorem toNat_insertLsb : (p.insertLsb b i).toNat = p.toNat.insertBit b i := rfl
+
+@[simp]
+theorem getElem_insertLsb_of_val_self : (p.insertLsb b i)[i.val] = b := Nat.testBit_insertBit_of_eq
+
+@[simp]
+theorem getElem_insertLsb_of_gt_val {j : ℕ} (hj : j < w + 1) :
+    ∀ (hij : i < j), (p.insertLsb b i)[j] = p[j - 1] := Nat.testBit_insertBit_of_gt
+@[simp]
+theorem getElem_insertLsb_of_lt_val {j : ℕ} (hj : j < w + 1) :
+    ∀ (hij : j < i), (p.insertLsb b i)[j] = p[j] := Nat.testBit_insertBit_of_lt
+
+@[grind =]
+theorem getElem_insertLsb {j : ℕ} (hj : j < w + 1) :
+    (p.insertLsb b i)[j] = if hij : i < j then p[j - 1] else if hij : j < i then p[j] else b := by
+  grind [getElem_insertLsb_of_val_self, getElem_insertLsb_of_gt_val, getElem_insertLsb_of_lt_val]
+
+@[grind =]
+theorem getElem?_insertLsb {j : ℕ} :
+    (p.insertLsb b i)[j]? = if hij : i < j then p[j - 1]? else if hij : j < i then p[j] else b := by
+  grind
+
+@[simps!]
+def removeLsb (q : BitVec (w + 1)) (i : Fin (w + 1)) : BitVec w :=
+  BitVec.ofNatLT (q.toNat.removeBit i) <|
+  (Nat.removeBit_lt_two_pow_iff_lt_two_pow i.is_le).mpr q.isLt
+
+variable {b : Bool} {q : BitVec (w + 1)} {p : BitVec w} {i : Fin (w + 1)}
+
+@[grind =]
+theorem toNat_removeLsb : (q.removeLsb i).toNat = q.toNat.removeBit i := rfl
+
+@[simp]
+theorem getElem_removeLsb_of_ge {j : ℕ} (hj : j < w) :
+    i ≤ j → (q.removeLsb i)[j] = q[j + 1] := Nat.testBit_removeBit_of_ge
+
+@[simp]
+theorem getElem_removeLsb_of_lt {j : ℕ} (hj : j < w) :
+    j < i → (q.removeLsb i)[j] = q[j] := Nat.testBit_removeBit_of_lt
+
+@[grind =]
+theorem getElem_removeLsb {j : ℕ} (hj : j < w) :
+    (q.removeLsb i)[j] = if i ≤ j then q[j + 1] else q[j] := by
+  grind [getElem_removeLsb_of_ge, getElem_removeLsb_of_lt]
+
+@[grind =]
+theorem getElem?_removeLsb {j : ℕ} :
+    (q.removeLsb i)[j]? = if hij : i ≤ j then q[j + 1]? else q[j] := by grind
+
+@[simp, grind =]
+theorem insertLsb_getElem_val_removeLsb_of_eq : (q.removeLsb i).insertLsb q[i.val] i = q :=
+  eq_of_toNat_eq Nat.insertBit_testBit_removeBit_of_eq
+
+@[simp, grind =]
+theorem removeLsb_insertLsb_of_eq : (p.insertLsb b i).removeLsb i = p :=
+  eq_of_toNat_eq Nat.removeBit_insertBit_of_eq
+
+@[simps! apply symm_apply]
+def insertLsbEquiv (i : Fin (w + 1)) : Bool × BitVec w ≃ BitVec (w + 1) where
+  toFun bp := bp.2.insertLsb bp.1 i
+  invFun n := (n[i.val], n.removeLsb i)
+  left_inv _ := by grind
+  right_inv _ := by grind
+
+theorem insertLsbEquiv_apply_toNat {bp} : ((insertLsbEquiv i) bp).toNat =
+    i.val.insertBitEquiv (bp.1, bp.2.toNat) := rfl
+
+theorem insertLsbEquiv_symm_apply_snd_toNat : ((insertLsbEquiv i).symm q).2.toNat =
+    (i.val.insertBitEquiv.symm q.toNat).2 := rfl
+
+end BitVec
